sf/Assignment07_01.v
@@ -11,13 +11,49 @@ Require Export Assignment07_00.
     it is sound.  Use the tacticals we've just seen to make the proof
     as elegant as possible. *)
 
+Theorem optimize_0plus_sound: forall a,
+  aeval (optimize_0plus a) = aeval a.
+Proof.
+  intros a. induction a.
+  Case "ANum". reflexivity.
+  Case "APlus". destruct a1.
+    SCase "a1 = ANum n". destruct n.
+      SSCase "n = 0".  simpl. apply IHa2.
+      SSCase "n <> 0". simpl. rewrite IHa2. reflexivity.
+    SCase "a1 = APlus a1_1 a1_2".
+      simpl. simpl in IHa1. rewrite IHa1.
+      rewrite IHa2. reflexivity.
+    SCase "a1 = AMinus a1_1 a1_2".
+      simpl. simpl in IHa1. rewrite IHa1.
+      rewrite IHa2. reflexivity.
+    SCase "a1 = AMult a1_1 a1_2".
+      simpl. simpl in IHa1. rewrite IHa1.
+      rewrite IHa2. reflexivity.
+  Case "AMinus".
+    simpl. rewrite IHa1. rewrite IHa2. reflexivity.
+  Case "AMult".
+    simpl. rewrite IHa1. rewrite IHa2. reflexivity.  Qed.
+
 Fixpoint optimize_0plus_b (b : bexp) : bexp :=
-  (* FILL IN HERE *) admit.
+  match b with
+  | BTrue => BTrue
+  | BFalse => BFalse
+  | BEq a1 a2 => BEq (optimize_0plus a1) (optimize_0plus a2)
+  | BLe a1 a2 => BLe (optimize_0plus a1) (optimize_0plus a2)
+  | BNot b' => BNot (optimize_0plus_b b')
+  | BAnd b1 b2 => BAnd (optimize_0plus_b b1) (optimize_0plus_b b2)
+  end.
 
 Theorem optimize_0plus_b_sound : forall b,
   beval (optimize_0plus_b b) = beval b.
 Proof.
-  (* FILL IN HERE *) admit.
+  intros. induction b.
+  reflexivity.
+  reflexivity.
+  simpl. repeat (rewrite optimize_0plus_sound). reflexivity.
+  simpl. repeat (rewrite optimize_0plus_sound). reflexivity.
+  simpl. rewrite IHb. reflexivity.
+  simpl. rewrite IHb1. rewrite IHb2. reflexivity.
 Qed.
 (** [] *)
 
