sf/Assignment07_03.v
@@ -8,13 +8,23 @@ Require Export Assignment07_02.
 
 
 Inductive bevalR: bexp -> bool -> Prop :=
-(* FILL IN HERE *)
-.
+  | E_BTrue : bevalR BTrue true
+  | E_BFalse : bevalR BFalse false
+  | E_BEq : forall (e1 e2 : aexp) (n1 n2 : nat), aevalR e1 n1 -> aevalR e2 n2 -> bevalR (BEq e1 e2) (beq_nat n1 n2)
+  | E_BLe : forall (e1 e2 : aexp) (n1 n2 : nat), aevalR e1 n1 -> aevalR e2 n2 -> bevalR (BLe e1 e2) (ble_nat n1 n2)
+  | E_BNot : forall (e : bexp) (b : bool), bevalR e b -> bevalR (BNot e) (negb b)
+  | E_BAnd : forall (e1 e2 : bexp) (b1 b2 : bool), bevalR e1 b1 -> bevalR e2 b2 -> bevalR (BAnd e1 e2) (andb b1 b2).
 
 Theorem beval_iff_bevalR : forall b bv,
   bevalR b bv <-> beval b = bv.
 Proof.
-  admit.
+  split.
+  - intros. induction H; try reflexivity;
+    try (simpl; try (rewrite aeval_iff_aevalR in *); subst; reflexivity).
+  - generalize dependent bv. induction b; try (simpl; intros; subst; constructor; try (rewrite aeval_iff_aevalR; reflexivity)).
+    apply IHb. reflexivity.
+    apply IHb1. reflexivity.
+    apply IHb2. reflexivity.
 Qed.
 
 (** [] *)
