sf/Assignment07_04.v
@@ -6,7 +6,8 @@ Require Export Assignment07_03.
 Lemma neq_id : forall (T:Type) x y (p q:T), x <> y -> 
                (if eq_id_dec x y then p else q) = q. 
 Proof.
-  (* FILL IN HERE *) admit.
+  intros. destruct (eq_id_dec x y).
+  tauto. reflexivity.
 Qed.
 (** [] *)
 
