sf/Assignment07_06.v
@@ -7,7 +7,8 @@ Theorem update_neq : forall x2 x1 n st,
   x2 <> x1 ->                        
   (update st x2 n) x1 = (st x1).
 Proof.
-  (* FILL IN HERE *) admit.
+  intros. unfold update. destruct (eq_id_dec x2 x1).
+  tauto. reflexivity.
 Qed.
 (** [] *)
 
